PREFIX prov: <http://www.w3.org/ns/prov#> 
PREFIX void: <http://rdfs.org/ns/void#> 
prefix rdf: <http://www.w3.org/1999/02/22-rdf-syntax-ns#> 
prefix rdfs: <http://www.w3.org/2000/01/rdf-schema#>
prefix prop-fr: <http://fr.dbpedia.org/property/>
prefix graph-fr:  <http://fr.dbpedia.org/graph/>
prefix abstract_graph: <http://fr.dbpedia.org/abstract_graph/>
PREFIX xsd: <https://www.w3.org/2001/XMLSchema#>

prop-fr:NbNotThing a rdf:Property;
    rdfs:domain    void:Dataset;
    rdfs:range  xsd:integer ;
    rdfs:label "Number of not owl:Thing objects"@en;
    rdfs:comment "Allows to compute the number of typed as more than a owl:Thing."@en.

#prop-fr:levelPartition a rdf:Property;
#    rdfs:subPropertyOf void:subset;
#    rdfs:domain    void:Dataset;
#    rdfs:range    void:Dataset;
#    rdfs:label "partition of heriarchy level"@en;
#    rdfs:comment "Allows to compute stats at a hierarchical level of the ontology"@en;

#prop-fr:level 
#    rdfs:domain    void:Dataset;
#    rdfs:range  xsd:integer ;
#    rdfs:label "ontological heriarchy level"@en;
#    rdfs:comment "level in a given ontological"@en;

<http://fr.dbpedia.org> void:subset abstract_graph:type_dbpediafr ;
    void:subset abstract_graph:type_wikidata;
    void:subset abstract_graph:type_dbpediafr_only;
    void:subset abstract_graph:type_wikidata_only;
    void:subset abstract_graph:prop-lit_dbpediafr;
    void:subset abstract_graph:prop-lit_wikidata;
    void:subset abstract_graph:prop-lit_dbpediafr_only;
    void:subset abstract_graph:prop-lit_wikidata_only;
    void:subset abstract_graph:prop-obj_dbpediafr;
    void:subset abstract_graph:prop-obj_wikidata;
    void:subset abstract_graph:prop-obj_dbpediafr_only;
    void:subset abstract_graph:prop-obj_wikidata_only;
    void:subset abstract_graph:mainclass_prop-lit_dbpediafr;
    void:subset abstract_graph:mainclass_prop-lit_dbpediafr_only;
    void:subset abstract_graph:mainclass_prop-lit_wikidata;
    void:subset abstract_graph:mainclass_prop-lit_wikidata_only;
    void:subset abstract_graph:mainclass_prop-obj_dbpediafr;
    void:subset abstract_graph:mainclass_prop-obj_dbpediafr_only;
    void:subset abstract_graph:mainclass_prop-obj_wikidata;
    void:subset abstract_graph:mainclass_prop-obj_wikidata_only.

##################### TYPES ABSTRACT GRAPHS
abstract_graph:type_dbpediafr  a prov:Entity,  void:Dataset.
abstract_graph:type_dbpediafr  prov:wasGeneratedBy <https://github.com/Wimmics/dbpedia-virtuoso-sparql-endpoint-quickstart/blob/master/dbpedia-loader/process/processStatsType.sh>, <https://github.com/Wimmics/dbpedia-virtuoso-sparql-endpoint-quickstart/blob/master/dbpedia-loader/process/processStatsTypeClassPart.sh>.
abstract_graph:type_dbpediafr  prov:wasDerivedFrom   graph-fr:dbpedia_mappings_instance-types, graph-fr:dbpedia_generic_page.
  abstract_graph:type_dbpediafr prov:qualifiedDerivation [
       a prov:Derivation;                      
       prov:entity  graph-fr:dbpedia_mappings_instance-types, graph-fr:dbpedia_generic_page;  
       rdfs:comment "This abstract graph is only used for statistics about types defined into Dbpedia type set";
       rdfs:label "Types defined in DBpedia Fr"@en;
       prov:hadUsage    graph-fr:statistics
    ].


abstract_graph:type_dbpediafr_only a prov:Entity, void:Dataset.
abstract_graph:type_dbpediafr_only  prov:wasGeneratedBy <https://github.com/Wimmics/dbpedia-virtuoso-sparql-endpoint-quickstart/blob/master/dbpedia-loader/process/processStatsType.sh>, <https://github.com/Wimmics/dbpedia-virtuoso-sparql-endpoint-quickstart/blob/master/dbpedia-loader/process/processStatsTypeClassPart.sh>.
abstract_graph:type_dbpediafr_only prov:wasDerivedFrom graph-fr:dbpedia_mappings_instance-types, graph-fr:dbpedia_generic_page.
abstract_graph:type_dbpediafr_only prov:wasInfluencedBy graph-fr:dbpedia_wikidata_instance-types.
abstract_graph:type_dbpediafr_only prov:qualifiedDerivation [
       a prov:Derivation;                      
       prov:entity     graph-fr:dbpedia_mappings_instance-types, graph-fr:dbpedia_generic_page;  
       rdfs:comment "This abstract graph is only used for statistics about triples defined into Dbpedia type set but not found into Wikidata"@en;
       rdfs:label "Triples about type only found in DBpedia Fr"@en;
       prov:hadUsage      graph-fr:statistics;
    ].

abstract_graph:type_wikidata a prov:Entity, void:Dataset.
abstract_graph:type_wikidata  prov:wasGeneratedBy <https://github.com/Wimmics/dbpedia-virtuoso-sparql-endpoint-quickstart/blob/master/dbpedia-loader/process/processStatsType.sh>, <https://github.com/Wimmics/dbpedia-virtuoso-sparql-endpoint-quickstart/blob/master/dbpedia-loader/process/processStatsTypeClassPart.sh>.
abstract_graph:type_wikidata prov:wasDerivedFrom graph-fr:dbpedia_wikidata_instance-types, graph-fr:dbpedia_generic_page.
abstract_graph:type_wikidata prov:qualifiedDerivation [
       a prov:Derivation;                      
       prov:entity     graph-fr:dbpedia_wikidata_instance-types, graph-fr:dbpedia_generic_page;  
       rdfs:comment "This abstract graph is only used for statistics about types defined into Wikidata type set";
       rdfs:label "Types defined in Wikidata"@en;
       prov:hadUsage      graph-fr:statistics;
    ].

abstract_graph:type_wikidata_only a prov:Entity, void:Dataset.
abstract_graph:type_wikidata_only  prov:wasGeneratedBy <https://github.com/Wimmics/dbpedia-virtuoso-sparql-endpoint-quickstart/blob/master/dbpedia-loader/process/processStatsType.sh>, <https://github.com/Wimmics/dbpedia-virtuoso-sparql-endpoint-quickstart/blob/master/dbpedia-loader/process/processStatsTypeClassPart.sh>.
abstract_graph:type_wikidata_only prov:wasDerivedFrom graph-fr:dbpedia_wikidata_instance-types, graph-fr:dbpedia_generic_page.
abstract_graph:type_dbpediafr_only prov:wasInfluencedBy graph-fr:dbpedia_mappings_instance-types.
abstract_graph:type_wikidata_only prov:qualifiedDerivation [
       a prov:Derivation;                      
       prov:entity     graph-fr:dbpedia_wikidata_instance-types, graph-fr:dbpedia_generic_page;  
       rdfs:comment "This abstract graph is only used for statistics triples defined into Wikidata but not found into DBPedia Fr";
       rdfs:label "Triples about type only found in Wikidata"@en;
       prov:hadUsage      graph-fr:statistics;
    ].

##################### PROP LIT ABSTRACT GRAPHS

abstract_graph:prop-lit_dbpediafr a prov:Entity, void:Dataset.
abstract_graph:prop-lit_dbpediafr prov:wasDerivedFrom graph-fr:dbpedia_mappings_mappingbased-literals, graph-fr:dbpedia_generic_page.
abstract_graph:prop-lit_dbpediafr  prov:wasGeneratedBy <https://github.com/Wimmics/dbpedia-virtuoso-sparql-endpoint-quickstart/blob/master/dbpedia-loader/process/processStatsPropLit.sh>.
abstract_graph:prop-lit_dbpediafr prov:qualifiedDerivation [
       a prov:Derivation;                      
       prov:entity     graph-fr:dbpedia_mappings_mappingbased-literals, graph-fr:dbpedia_generic_page;  
       rdfs:comment "This abstract graph is only used for statistics about properties with litterals values defined into Dbpedia Fr";
       rdfs:label "Triples related to properties with literal values in DBpedia"@en;
       prov:hadUsage      graph-fr:statistics;
    ].

abstract_graph:prop-lit_dbpediafr_only a prov:Entity, void:Dataset.
abstract_graph:prop-lit_dbpediafr_only prov:wasDerivedFrom graph-fr:dbpedia_mappings_mappingbased-literals, graph-fr:dbpedia_generic_page.
abstract_graph:prop-lit_dbpediafr_only  prov:wasGeneratedBy <https://github.com/Wimmics/dbpedia-virtuoso-sparql-endpoint-quickstart/blob/master/dbpedia-loader/process/processStatsPropLit.sh>.
abstract_graph:type_dbpediafr_only prov:wasInfluencedBy graph-fr:dbpedia_wikidata_mappingbased-literals.
abstract_graph:prop-lit_dbpediafr_only prov:qualifiedDerivation [
       a prov:Derivation;                      
       prov:entity     graph-fr:dbpedia_mappings_mappingbased-literals, graph-fr:dbpedia_generic_page;  
       rdfs:comment "This abstract graph is only used for statistics about properties with litterals values defined into Dbpedia Fr and not into Wikidata";
       rdfs:label "Triples related to properties with literal values in DBpedia and not in Wikidata"@en;
       prov:hadUsage      graph-fr:statistics;
    ].

abstract_graph:prop-lit_wikidata a prov:Entity, void:Dataset.
abstract_graph:prop-lit_wikidata prov:wasDerivedFrom graph-fr:dbpedia_wikidata_mappingbased-literals, graph-fr:dbpedia_generic_page.
abstract_graph:prop-lit_wikidata  prov:wasGeneratedBy <https://github.com/Wimmics/dbpedia-virtuoso-sparql-endpoint-quickstart/blob/master/dbpedia-loader/process/processStatsPropLit.sh>.
abstract_graph:prop-lit_wikidata prov:qualifiedDerivation [
       a prov:Derivation;                      
       prov:entity     graph-fr:dbpedia_wikidata_mappingbased-literals, graph-fr:dbpedia_generic_page;  
       rdfs:comment "This abstract graph is only used for statistics about properties with litterals values defined into Wikidata";
       rdfs:label "Triples related to properties with literal values in DBpedia Fr"@en;
       prov:hadUsage      graph-fr:statistics;
    ].

abstract_graph:prop-lit_wikidata_only a prov:Entity, void:Dataset.
abstract_graph:prop-lit_wikidata_only  prov:wasGeneratedBy <https://github.com/Wimmics/dbpedia-virtuoso-sparql-endpoint-quickstart/blob/master/dbpedia-loader/process/processStatsPropLit.sh>.
abstract_graph:prop-lit_wikidata_only prov:wasDerivedFrom graph-fr:dbpedia_wikidata_mappingbased-literals, graph-fr:dbpedia_generic_page.
abstract_graph:prop-lit_wikidata_only prov:qualifiedDerivation [
       a prov:Derivation;                      
       prov:entity     graph-fr:dbpedia_wikidata_mappingbased-literals, graph-fr:dbpedia_generic_page;  
       rdfs:comment "This abstract graph is only used for statistics about properties with litterals values defined into Wikidata and not into Dbpedia Fr";
       rdfs:label "Triples related to properties with literal values in Wikidata and not in DBpedia Fr"@en;
       prov:hadUsage      graph-fr:statistics;
    ].

##################### PROP OBJ ABSTRACT GRAPHS

abstract_graph:prop-obj_dbpediafr a prov:Entity, void:Dataset.
abstract_graph:prop-obj_dbpediafr  prov:wasGeneratedBy <https://github.com/Wimmics/dbpedia-virtuoso-sparql-endpoint-quickstart/blob/master/dbpedia-loader/process/processStatsPropObj.sh>.
abstract_graph:prop-obj_dbpediafr prov:wasDerivedFrom graph-fr:dbpedia_mappings_mappingbased-objects-uncleaned, graph-fr:dbpedia_generic_page.
abstract_graph:prop-obj_dbpediafr prov:qualifiedDerivation [
       a prov:Derivation;                      
       prov:entity     graph-fr:dbpedia_mappings_mappingbased-objects-uncleaned, graph-fr:dbpedia_generic_page;  
       rdfs:comment "This abstract graph is only used for statistics about properties with object values defined into Dbpedia Fr";
       rdfs:label "Triples related to properties with literal values in DBpedia"@en;
       prov:hadUsage      graph-fr:statistics;
    ].

abstract_graph:prop-obj_dbpediafr_only a prov:Entity, void:Dataset.
abstract_graph:prop-obj_dbpediafr_only prov:wasDerivedFrom graph-fr:dbpedia_mappings_mappingbased-objects-uncleaned, graph-fr:dbpedia_generic_page.
abstract_graph:prop-obj_dbpediafr_only  prov:wasGeneratedBy <https://github.com/Wimmics/dbpedia-virtuoso-sparql-endpoint-quickstart/blob/master/dbpedia-loader/process/processStatsPropObj.sh>.
abstract_graph:type_dbpediafr_only prov:wasInfluencedBy graph-fr:dbpedia_wikidata_mappingbased-literals.
abstract_graph:prop-obj_dbpediafr_only prov:qualifiedDerivation [
       a prov:Derivation;                      
       prov:entity     graph-fr:dbpedia_mappings_mappingbased-objects-uncleaned, graph-fr:dbpedia_generic_page;  
       rdfs:comment "This abstract graph is only used for statistics about properties with object values defined into Dbpedia Fr and not into Wikidata";
       rdfs:label "Triples related to properties with literal values in DBpedia and not in Wikidata"@en;
       prov:hadUsage      graph-fr:statistics;
    ].

abstract_graph:prop-obj_wikidata a prov:Entity, void:Dataset.
abstract_graph:prop-obj_wikidata prov:wasDerivedFrom graph-fr:dbpedia_wikidata_mappingbased-objects-uncleaned, graph-fr:dbpedia_generic_page.
abstract_graph:prop-obj_wikidata  prov:wasGeneratedBy <https://github.com/Wimmics/dbpedia-virtuoso-sparql-endpoint-quickstart/blob/master/dbpedia-loader/process/processStatsPropObj.sh>.
abstract_graph:prop-obj_wikidata prov:qualifiedDerivation [
       a prov:Derivation;                      
       prov:entity     graph-fr:dbpedia_wikidata_mappingbased-objects-uncleaned, graph-fr:dbpedia_generic_page;  
       rdfs:comment "This abstract graph is only used for statistics about properties with object values defined into Wikidata";
       rdfs:label "Triples related to properties with literal values in DBpedia Fr"@en;
       prov:hadUsage      graph-fr:statistics;
    ].

abstract_graph:prop-obj_wikidata_only a prov:Entity, void:Dataset.
abstract_graph:prop-obj_wikidata_only prov:wasDerivedFrom graph-fr:dbpedia_wikidata_mappingbased-objects-uncleaned, graph-fr:dbpedia_generic_page.
abstract_graph:prop-obj_wikidata_only  prov:wasGeneratedBy <https://github.com/Wimmics/dbpedia-virtuoso-sparql-endpoint-quickstart/blob/master/dbpedia-loader/process/processStatsPropObj.sh>.
abstract_graph:type_dbpediafr_only prov:wasInfluencedBy graph-fr:dbpedia_mappings_mappingbased-objects-uncleaned.
abstract_graph:prop-obj_wikidata_only prov:qualifiedDerivation [
       a prov:Derivation;                      
       prov:entity     graph-fr:dbpedia_wikidata_mappingbased-objects-uncleaned, graph-fr:dbpedia_generic_page;  
       rdfs:comment "This abstract graph is only used for statistics about properties with object values defined into Wikidata and not into Dbpedia Fr";
       rdfs:label "Triples related to properties with literal values in Wikidata and not in DBpedia Fr"@en;
       prov:hadUsage      graph-fr:statistics;
    ].



##################### MAIN CLASS ABSTRACT GRAPHS - PROP LIT

abstract_graph:mainclass_prop-lit_dbpediafr a prov:Entity, void:Dataset.
abstract_graph:mainclass_prop-lit_dbpediafr  prov:wasGeneratedBy <https://github.com/Wimmics/dbpedia-virtuoso-sparql-endpoint-quickstart/blob/master/dbpedia-loader/process/processStatsMainClass.sh>.
abstract_graph:mainclass_prop-lit_dbpediafr prov:wasDerivedFrom graph-fr:dbpedia_mappings_mappingbased-literals, graph-fr:dbpedia_generic_page, graph-fr:dbpedia_mappings_instance-types.
abstract_graph:mainclass_prop-lit_dbpediafr prov:qualifiedDerivation [
       a prov:Derivation;                      
       prov:entity     graph-fr:dbpedia_mappings_mappingbased-literals, graph-fr:dbpedia_generic_page, graph-fr:dbpedia_mappings_instance-types;
       rdfs:comment "This abstract graph is only used for statistics computed on the main class of the DBpedia Ontology on properties with lit value defined in DBpedia Fr";
       rdfs:label "Main class properties with literal values stats"@en;
       prov:hadUsage      graph-fr:statistics;
    ].

abstract_graph:mainclass_prop-lit_dbpediafr_only a prov:Entity, void:Dataset.
abstract_graph:mainclass_prop-lit_dbpediafr_only  prov:wasGeneratedBy <https://github.com/Wimmics/dbpedia-virtuoso-sparql-endpoint-quickstart/blob/master/dbpedia-loader/process/processStatsMainClass.sh>.
abstract_graph:mainclass_prop-lit_dbpediafr_only prov:wasDerivedFrom graph-fr:dbpedia_mappings_mappingbased-literals, graph-fr:dbpedia_generic_page, graph-fr:dbpedia_mappings_instance-types.
abstract_graph:mainclass_prop-lit_dbpediafr_only prov:wasInfluencedBy graph-fr:dbpedia_wikidata_mappingbased-literals.
abstract_graph:mainclass_prop-lit_dbpediafr_only prov:qualifiedDerivation [
       a prov:Derivation;                      
       prov:entity     graph-fr:dbpedia_mappings_mappingbased-literals, graph-fr:dbpedia_generic_page, graph-fr:dbpedia_mappings_instance-types;
       rdfs:comment "This abstract graph is only used for statistics computed on the main class of the DBpedia Ontology on properties with lit value where triples only appears in DBpedia";
       rdfs:label "Main class properties with literal values stats"@en;
       prov:hadUsage      graph-fr:statistics;
    ].

abstract_graph:mainclass_prop-lit_wikidata a prov:Entity, void:Dataset.
abstract_graph:mainclass_prop-lit_wikidata  prov:wasGeneratedBy <https://github.com/Wimmics/dbpedia-virtuoso-sparql-endpoint-quickstart/blob/master/dbpedia-loader/process/processStatsMainClass.sh>.
abstract_graph:mainclass_prop-lit_wikidata prov:wasDerivedFrom graph-fr:dbpedia_mappings_mappingbased-literals, graph-fr:dbpedia_generic_page, graph-fr:dbpedia_wikidata_mappingbased-literals.
abstract_graph:mainclass_prop-lit_wikidata prov:qualifiedDerivation [
       a prov:Derivation;                      
       prov:entity     graph-fr:dbpedia_mappings_mappingbased-literals, graph-fr:dbpedia_generic_page, graph-fr:dbpedia_mappings_instance-types;
       rdfs:comment "This abstract graph is only used for statistics computed on the main class of the DBpedia Ontology on properties with lit value defined in Wikidata";
       rdfs:label "Main class properties with literal values stats"@en;
       prov:hadUsage      graph-fr:statistics;
    ].

abstract_graph:mainclass_prop-lit_wikidata_only a prov:Entity, void:Dataset.
abstract_graph:mainclass_prop-lit_wikidata_only  prov:wasGeneratedBy <https://github.com/Wimmics/dbpedia-virtuoso-sparql-endpoint-quickstart/blob/master/dbpedia-loader/process/processStatsMainClass.sh>.
abstract_graph:mainclass_prop-lit_wikidata_only prov:wasDerivedFrom graph-fr:dbpedia_wikidata_mappingbased-literals, graph-fr:dbpedia_generic_page, graph-fr:dbpedia_mappings_instance-types.
abstract_graph:mainclass_prop-lit_wikidata_only prov:wasInfluencedBy graph-fr:dbpedia_mappings_mappingbased-literals.
abstract_graph:mainclass_prop-lit_wikidata_only prov:qualifiedDerivation [
       a prov:Derivation;                      
       prov:entity     graph-fr:dbpedia_mappings_mappingbased-literals, graph-fr:dbpedia_generic_page, graph-fr:dbpedia_mappings_instance-types;
       rdfs:comment "This abstract graph is only used for statistics computed on the main class of the DBpedia Ontology on properties with lit value where triples only appears in DBpedia";
       rdfs:label "Main class properties with literal values stats"@en;
       prov:hadUsage      graph-fr:statistics;
    ].



##################### MAIN CLASS ABSTRACT GRAPHS - PROP OBJ

abstract_graph:mainclass_prop-obj_dbpediafr a prov:Entity, void:Dataset.
abstract_graph:mainclass_prop-obj_dbpediafr  prov:wasGeneratedBy <https://github.com/Wimmics/dbpedia-virtuoso-sparql-endpoint-quickstart/blob/master/dbpedia-loader/process/processStatsMainClass.sh>.
abstract_graph:mainclass_prop-obj_dbpediafr prov:wasDerivedFrom graph-fr:dbpedia_mappings_mappingbased-objects-uncleaned, graph-fr:dbpedia_generic_page, graph-fr:dbpedia_mappings_instance-types.
abstract_graph:mainclass_prop-obj_dbpediafr prov:qualifiedDerivation [
       a prov:Derivation;                      
       prov:entity     graph-fr:dbpedia_mappings_mappingbased-objects-uncleaned, graph-fr:dbpedia_generic_page, graph-fr:dbpedia_mappings_instance-types;
       rdfs:comment "This abstract graph is only used for statistics computed on the main class of the DBpedia Ontology on properties with lit value defined in DBpedia Fr";
       rdfs:label "Main class properties with literal values stats"@en;
       prov:hadUsage      graph-fr:statistics;
    ].

abstract_graph:mainclass_prop-obj_dbpediafr_only a prov:Entity, void:Dataset.
abstract_graph:mainclass_prop-obj_dbpediafr_only  prov:wasGeneratedBy <https://github.com/Wimmics/dbpedia-virtuoso-sparql-endpoint-quickstart/blob/master/dbpedia-loader/process/processStatsMainClass.sh>.
abstract_graph:mainclass_prop-obj_dbpediafr_only prov:wasDerivedFrom graph-fr:dbpedia_mappings_mappingbased-objects-uncleaned, graph-fr:dbpedia_generic_page, graph-fr:dbpedia_mappings_instance-types.
abstract_graph:mainclass_prop-obj_dbpediafr_only prov:wasInfluencedBy graph-fr:dbpedia_wikidata_mappingbased-objects-uncleaned.
abstract_graph:mainclass_prop-obj_dbpediafr_only prov:qualifiedDerivation [
       a prov:Derivation;                      
       prov:entity     graph-fr:dbpedia_mappings_mappingbased-objects-uncleaned, graph-fr:dbpedia_generic_page, graph-fr:dbpedia_mappings_instance-types;
       rdfs:comment "This abstract graph is only used for statistics computed on the main class of the DBpedia Ontology on properties with lit value where triples only appears in DBpedia";
       rdfs:label "Main class properties with literal values stats"@en;
       prov:hadUsage      graph-fr:statistics;
    ].

abstract_graph:mainclass_prop-obj_wikidata a prov:Entity, void:Dataset.
abstract_graph:mainclass_prop-obj_wikidata  prov:wasGeneratedBy <https://github.com/Wimmics/dbpedia-virtuoso-sparql-endpoint-quickstart/blob/master/dbpedia-loader/process/processStatsMainClass.sh>.
abstract_graph:mainclass_prop-obj_wikidata prov:wasDerivedFrom graph-fr:dbpedia_wikidata_mappingbased-objects-uncleaned, graph-fr:dbpedia_generic_page, graph-fr:dbpedia_wikidata_mappingbased-literals.
abstract_graph:mainclass_prop-obj_wikidata prov:qualifiedDerivation [
       a prov:Derivation;                      
       prov:entity     graph-fr:dbpedia_wikidata_mappingbased-objects-uncleaned, graph-fr:dbpedia_generic_page, graph-fr:dbpedia_mappings_instance-types;
       rdfs:comment "This abstract graph is only used for statistics computed on the main class of the DBpedia Ontology on properties with lit value defined in Wikidata";
       rdfs:label "Main class properties with literal values stats"@en;
       prov:hadUsage      graph-fr:statistics;
    ].

abstract_graph:mainclass_prop-obj_wikidata_only a prov:Entity, void:Dataset.
abstract_graph:mainclass_prop-obj_wikidata_only  prov:wasGeneratedBy <https://github.com/Wimmics/dbpedia-virtuoso-sparql-endpoint-quickstart/blob/master/dbpedia-loader/process/processStatsMainClass.sh>.
abstract_graph:mainclass_prop-obj_wikidata_only prov:wasDerivedFrom graph-fr:dbpedia_wikidata_mappingbased-objects-uncleaned, graph-fr:dbpedia_generic_page, graph-fr:dbpedia_mappings_instance-types.
abstract_graph:mainclass_prop-obj_wikidata_only prov:wasInfluencedBy graph-fr:dbpedia_mappings_mappingbased-objects-uncleaned.
abstract_graph:mainclass_prop-obj_wikidata_only prov:qualifiedDerivation [
       a prov:Derivation;                      
       prov:entity     graph-fr:dbpedia_wikidata_mappingbased-objects-uncleaned, graph-fr:dbpedia_generic_page, graph-fr:dbpedia_mappings_instance-types;
       rdfs:comment "This abstract graph is only used for statistics computed on the main class of the DBpedia Ontology on properties with lit value where triples only appears in DBpedia";
       rdfs:label "Main class properties with literal values stats"@en;
       prov:hadUsage      graph-fr:statistics;
    ].
